automat/CaseStudy/medUnfairStep.thy
@@ -6,20 +6,12 @@ begin
 
 
 (* counter not null, drop every message and count one down *)
-lemma "spsConcIn (medIn (Msg m)) (medUnfair (Suc n)) = spsConcOut (medOut -)(medUnfair n)"
+lemma "spsConcIn (medIn (Msg m)) (medUnfair) = spsConcOut (medOut -)(medUnfair)"
   oops
 
 (* If a "null" comes in send it out and stay in the same state *) 
-lemma "spsConcIn (medIn -) (medUnfair state) = spsConcOut (medOut -)(medUnfair state)"
+lemma "spsConcIn (medIn -) (medUnfair) = spsConcOut (medOut -)(medUnfair)"
   oops
-
-(* Counter hit zero, so pass the message and reset the countdown to a random value *)
-lemma "spsConcIn (medIn (Msg m)) (medUnfair 0) 
-  = uspecUnion\<cdot>
-      (spsConcOut (medOut (Msg m))(uspecFlatten medInDom medOutDom (Rev {medUnfair n |  n. True})))\<cdot>
-      (spsConcOut (medOut (Msg m))(medUnfair 0))"
-  oops
-
 
 lemma "uspecIsConsistent (medUnfair state)"
   oops  (* ToDo: Prove this by using the consistent lemma over medFair *)
